Kura/Graph/Subgraph.lean
@@ -6,48 +6,61 @@ open edge
 variable {V W E F : Type*} [LinearOrder V] [LinearOrder W]
 
 
+/--
+If removeV v = true, v is removed when InducedSubgraph is evaluated-/
 structure InducedSubgraph (G : Graph V E) where
-  rmv : V → Bool
+  Vset : Set V
+  DecVMem : DecidablePred (· ∈ Vset)
 
 structure Subgraph (G : Graph V E) extends InducedSubgraph G where
-  rme : E → Bool
-  hrme : ∀ e v, rmv v → v ∈ G.inc e → rme e
+  Eset : Set E
+  DecEMem : DecidablePred (· ∈ Eset)
+  Eset_spec : ∀ e ∈ Eset, ∀ v ∈ G.inc e, v ∈ Vset
 
 structure QuotientGraph (G : Graph V E) where
   vmap : V → V
   vmap_idem : ∀ v, vmap (vmap v) = vmap v
 
-structure QuotientInducedSubgraph (G : Graph V E) extends InducedSubgraph G where
-  vmap : V → WithBot V
-  vmap_dom : ∀ v, ¬rmv v ↔ (vmap v).isSome
-  vmap_ran : ∀ v, (hdom : ¬rmv v) → ¬ rmv ((vmap v).get ((vmap_dom v).mp hdom))
-  vmap_idem : ∀ v, (hdom : ¬rmv v) → vmap ((vmap v).get ((vmap_dom v).mp hdom)) = vmap v
+/-- If v is mapped to ⊥ = none, remove it -/
+structure QuotientSubgraph (G : Graph V E) where
+  vmap' : V → WithBot V
+  vmap'_idem : ∀ v, Option.bind (vmap' v) vmap' = vmap' v
+  Eset : Set E
+  DecEMem : DecidablePred (· ∈ Eset)
+  Eset_spec : ∀ e v, vmap' v = ⊥ → v ∈ G.inc e → e ∉ Eset
 
-structure QuotientSubgraph (G : Graph V E) extends Subgraph G, QuotientInducedSubgraph G where
+----------------------------------------------------------------------
+-- useful lemma
 
-def deleteEdges (G: Graph V E) (S : Set E) [DecidablePred (· ∈ S)] : Subgraph G where
-  rmv := fun _ ↦ false
-  rme := fun e : E ↦ if (e ∈ S) then true else false
-  hrme := by
-    simp only [Bool.false_eq_true, Bool.if_false_right, Bool.and_true, decide_eq_true_eq,
-      false_implies, implies_true]
+variable {G : Graph V E}
 
+lemma Subgraph.not_mem_Eset  (S : Subgraph G) (he : ∃ v ∈ G.inc e, v ∉ S.Vset) :
+    e ∉ S.Eset := by
+  intro h
+  absurd S.Eset_spec e h
+  push_neg
+  exact he
 
-lemma Subgraph.hrme' {G : Graph V E} (S : Subgraph G) (e : E) (he : ¬S.rme e) :
-    ∀ v ∈ G.inc e, ¬S.rmv v := fun _ hv hvrm => he (S.hrme _ _ hvrm hv)
+/-- Expose the decidability of (· ∈ Vset) -/
+instance InducedSubgraphDecVMem {G : Graph V E} (S : InducedSubgraph G) :
+    DecidablePred (· ∈ S.Vset) := S.DecVMem
 
+/-- Expose the decidability of (· ∈ Eset)-/
+instance SubgraphDecEMem (S : Subgraph G) : DecidablePred (· ∈ S.Eset) := S.DecEMem
+
+/-- Make vmap_idem simp-avaliable-/
 @[simp]
-def QuotientGraph.vmap_idem_for_simp {G : Graph V E} (S : QuotientGraph G) (v : V) :
+lemma QuotientGraph.vmap_idem_for_simp  (S : QuotientGraph G) (v : V) :
     S.vmap (S.vmap v) = S.vmap v := S.vmap_idem v
 
-def QuotientGraph.ran {G : Graph V E} (S : QuotientGraph G) : Set V :=
+def QuotientGraph.ran (S : QuotientGraph G) : Set V :=
   {v | ∃ u, S.vmap u = v}
 
-lemma QuotientGraph.mem_ran_iff {G : Graph V E} (S : QuotientGraph G) (v : V) :
+lemma QuotientGraph.mem_ran_iff (S : QuotientGraph G) (v : V) :
     v ∈ S.ran ↔ ∃ u, S.vmap u = v := Iff.rfl
 
 @[simp]
-lemma QuotientGraph.mem_ran_iff_vmap_self {G : Graph V E} (S : QuotientGraph G) (v : V) :
+lemma QuotientGraph.mem_ran_iff_vmap_self (S : QuotientGraph G) (v : V) :
     v ∈ S.ran ↔ S.vmap v = v := by
   rw [QuotientGraph.mem_ran_iff]
   constructor
@@ -57,156 +70,160 @@ lemma QuotientGraph.mem_ran_iff_vmap_self {G : Graph V E} (S : QuotientGraph G) 
   · rintro h
     exact ⟨ v, h ⟩
 
-def QuotientGraph.vmap' {G : Graph V E} (S : QuotientGraph G) (v : V) : S.ran :=
+def QuotientGraph.vmap' (S : QuotientGraph G) (v : V) : S.ran :=
   ⟨ S.vmap v, by rw [mem_ran_iff_vmap_self, vmap_idem_for_simp]⟩
 
-def QuotientInducedSubgraph.ran {G : Graph V E} (S : QuotientInducedSubgraph G) : Set V :=
-  {v | ∃ u, S.rmv u ∧ S.vmap u = some v}
+def QuotientSubgraph.ran (S : QuotientSubgraph G) : Set V :=
+  {v | ∃ u, S.vmap' u = some v}
 
 
-def InducedSubgraph.eval {G : Graph V E} (S : InducedSubgraph G) :
-  Graph {v : V // ¬S.rmv v} {e // (G.inc e).all (¬S.rmv ·) } where
+-------------------------------------------------
+-- Evaluations
+
+def InducedSubgraph.eval (S : InducedSubgraph G) :
+  Graph S.Vset {e // (G.inc e).all (· ∈ S.Vset) } where
   inc e := edge.pmap Subtype.mk (G.inc e.1) (by
-    simpa only [Bool.not_eq_true, Bool.decide_eq_false, all_iff, Bool.not_eq_true'] using e.prop)
+    simpa only [all_iff, decide_eq_true_eq] using e.prop)
 
-def Subgraph.eval {G : Graph V E} (S : Subgraph G) :
-  Graph {v : V // ¬S.rmv v} {e // ¬S.rme e ∧ (G.inc e).all (¬S.rmv ·)} where
-  inc e := edge.pmap Subtype.mk (G.inc e.1) (by
-    simpa only [Bool.not_eq_true, Bool.decide_eq_false, all_iff, Bool.not_eq_true'] using e.2.2)
+def Subgraph.eval (S : Subgraph G) :
+  Graph S.Vset S.Eset where
+  inc e := edge.pmap Subtype.mk (G.inc e.1) (S.Eset_spec e.val e.prop)
 
-def QuotientGraph.eval {G : Graph V E} (S : QuotientGraph G) : Graph (S.ran) E where
+def QuotientGraph.eval (S : QuotientGraph G) : Graph (S.ran) E where
   inc e := (G.inc e).map S.vmap'
 
 instance InducedSubgraphFullgraph [fullGraph G] (S : InducedSubgraph G) :
-  fullGraph (V := {v : V // ¬S.rmv v}) S.eval where
+  fullGraph (V := S.Vset) S.eval where
   all_full := sorry
 
 instance SubgraphFullgraph [fullGraph G] (S : Subgraph G) :
-  fullGraph (V := {v : V // ¬S.rmv v}) S.eval where
+  fullGraph (V := S.Vset) S.eval where
   all_full := sorry
 
 instance InducedSubgraphUndirected [Undirected G] (S : InducedSubgraph G) :
-  Undirected (V := {v : V // ¬S.rmv v}) S.eval where
+  Undirected (V := S.Vset) S.eval where
   edge_symm := sorry
 
 instance SubgraphUndirected [Undirected G] (S : Subgraph G) :
-  Undirected (V := {v : V // ¬S.rmv v}) S.eval where
+  Undirected (V := S.Vset) S.eval where
   edge_symm := sorry
 
 
+-----------------------------------------------------------------------------
+-- Initializations
+
 variable (G : Graph V E)
 
-def InducedSubgraph.init : InducedSubgraph G := { rmv := fun _ => false }
+def InducedSubgraph.init : InducedSubgraph G where
+  Vset := Set.univ
+  DecVMem := by infer_instance
 
 def Subgraph.init : Subgraph G where
-  rmv := fun _ => false
-  rme := fun _ => false
-  hrme := by
-    simp only [Bool.false_eq_true, imp_false, false_implies, implies_true]
+  Vset := Set.univ
+  DecVMem := by infer_instance
+  Eset := Set.univ
+  DecEMem := by infer_instance
+  Eset_spec := by simp only [Set.mem_univ, implies_true, imp_self]
 
 def QuotientGraph.init : QuotientGraph G where
   vmap := id
   vmap_idem := fun _ => rfl
 
-def QuotientInducedSubgraph.init : QuotientInducedSubgraph G where
-  rmv := fun _ => false
-  vmap := some
-  vmap_dom := by
-    simp only [Bool.false_eq_true, not_false_eq_true, Option.isSome_some, implies_true]
-  vmap_ran := fun u => id
-  vmap_idem := by
-    simp only [Option.get_some, implies_true]
-
 def QuotientSubgraph.init : QuotientSubgraph G where
-  toSubgraph := Subgraph.init G
-  vmap := some
-  vmap_dom := by simp only [Subgraph.init, Bool.false_eq_true, not_false_eq_true,
-    Option.isSome_some, implies_true]
-  vmap_ran := fun u => id
-  vmap_idem := by simp only [Option.get_some, implies_true]
+  vmap' := some
+  vmap'_idem := by simp only [Option.bind_some, implies_true]
+  Eset := Set.univ
+  DecEMem := by infer_instance
+  Eset_spec := by simp only [reduceCtorEq, Set.mem_univ, not_true_eq_false, imp_false,
+    false_implies, implies_true]
 
+-----------------------------------------------------------------------------
+-- Elementary operations
 
 variable {G : Graph V E}
 
 def InducedSubgraph.vrm (G' : InducedSubgraph G) (v : V) : InducedSubgraph G where
-  rmv u := u = v || G'.rmv u
+  Vset := G'.Vset \ {v}
+  DecVMem := by infer_instance
 
-def InducedSubgraph.vrmFinset (G' : InducedSubgraph G) (S : Finset V) : InducedSubgraph G where
-  rmv u := u ∈ S || G'.rmv u
+def InducedSubgraph.OnSet (G' : InducedSubgraph G) (S : Set V) [DecidablePred (· ∈ S)] :
+    InducedSubgraph G where
+  Vset := G'.Vset ∩ S
+  DecVMem := by infer_instance
 
-def InducedSubgraph.OnFinset (G' : InducedSubgraph G) (S : Finset V) : InducedSubgraph G where
-  rmv u := u ∉ S || G'.rmv u
+macro G:term "[" S:term "]" : term =>
+  `(InducedSubgraph.eval (InducedSubgraph.OnSet (InducedSubgraph.init $G) $S))
 
-macro G:term "[" S:term "]" : term => `(InducedSubgraph.eval (InducedSubgraph.OnFinset (InducedSubgraph.init $G) $S))
 
 def Subgraph.vrm (G' : Subgraph G) (v : V) : Subgraph G where
-  rmv u := u = v || G'.rmv u
-  rme e := v ∈ G.inc e || G'.rme e
-  hrme := by
-    intro e v' hv' hv'e
-    simp only [Bool.or_eq_true, decide_eq_true_eq] at hv' ⊢
-    rcases hv' with rfl | h
-    · exact Or.inl hv'e
-    · exact Or.inr (G'.hrme _ _ h hv'e)
+  Vset := G'.Vset \ {v}
+  DecVMem := by infer_instance
+  Eset := {e ∈ G'.Eset | G.all e (· ≠ v)}
+  DecEMem := by infer_instance
+  Eset_spec e he u hu := by
+    simp only [all, ne_eq, decide_not, all_iff, Bool.not_eq_true', decide_eq_false_iff_not,
+      Set.mem_setOf_eq, Set.mem_diff, Set.mem_singleton_iff] at he ⊢
+    constructor
+    · exact G'.Eset_spec e he.1 u hu
+    · exact he.2 u hu
+
+def Subgraph.OnSetV (G' : Subgraph G) (S : Set V) [DecidablePred (· ∈ S)] : Subgraph G where
+  Vset := G'.Vset ∩ S
+  DecVMem := by infer_instance
+  Eset := {e ∈ G'.Eset | G.all e (· ∈ S)}
+  DecEMem := by infer_instance
+  Eset_spec e he u hu := by
+    simp only [all, all_iff, decide_eq_true_eq, Set.mem_setOf_eq, Set.mem_inter_iff] at he ⊢
+    constructor
+    · exact G'.Eset_spec e he.1 u hu
+    · exact he.2 u hu
 
 def Subgraph.erm [DecidableEq E] (G' : Subgraph G) (e : E) : Subgraph G where
-  rmv := G'.rmv
-  rme e' := e = e' || G'.rme e'
-  hrme := fun v e hv hv'e => by
-    rw [Bool.or_eq_true, decide_eq_true_eq]
-    exact Or.inr (G'.hrme v e hv hv'e)
+  Vset := G'.Vset
+  DecVMem := by infer_instance
+  Eset := G'.Eset \ {e}
+  DecEMem := by infer_instance
+  Eset_spec e' he' u hu := by
+    simp only [Set.mem_diff, Set.mem_singleton_iff] at he'
+    exact G'.Eset_spec e' he'.1 u hu
 
-lemma Subgraph.not_mem_erm [DecidableEq E] [fullGraph G]
-  (G' : Subgraph G) (e : E) (he : ¬G'.rme e) :
-    let G'' := G'.erm e
-    ¬ (¬G''.rme e ∧ (G.inc e).all (¬G''.rmv ·)) := by
-  sorry
+def Subgraph.OnSetE (G' : Subgraph G) (S : Set E) [DecidablePred (· ∈ S)] : Subgraph G where
+  Vset := G'.Vset
+  DecVMem := by infer_instance
+  Eset := G'.Eset ∩ S
+  DecEMem := by infer_instance
+  Eset_spec e he u hu := by
+    simp only [Set.mem_inter_iff] at he
+    exact G'.Eset_spec e he.1 u hu
+
+macro G:term "{" S:term "}" : term => `(Subgraph.eval (Subgraph.OnSetE (Subgraph.init $G) $S))
 
 /-- The second vertex is being merged into the first vertex-/
 def QuotientGraph.merge (G' : QuotientGraph G) (v w : V) :
     QuotientGraph G where
   vmap u := if G'.vmap u = w then G'.vmap v else G'.vmap u
   vmap_idem u := by
-    simp only
-    by_cases hu : G'.vmap u = w
-    · subst hu
-      simp only [↓reduceIte, vmap_idem_for_simp, ite_self]
-    · simp only [hu, ↓reduceIte, vmap_idem_for_simp]
+    by_cases hu : G'.vmap u = w <;> simp only [hu, ↓reduceIte, vmap_idem_for_simp, ite_self]
 
-def QuotientGraph.mergeSetOn (G' : QuotientGraph G) (P : V → Prop) [DecidablePred P] (x : V) :
+def QuotientGraph.mergeOnSet (G' : QuotientGraph G) (S : Set V) [DecidablePred (· ∈ S)] (x : V) :
     QuotientGraph G where
-  vmap u := if P (G'.vmap u) then G'.vmap x else G'.vmap u
+  vmap u := if G'.vmap u ∈ S then G'.vmap x else G'.vmap u
   vmap_idem u := by
-    simp only
-    by_cases hu : P (G'.vmap u)
-    · simp only [hu, ↓reduceIte, vmap_idem_for_simp, ite_self]
-    · simp only [hu, ↓reduceIte, vmap_idem_for_simp]
+    by_cases hu : G'.vmap u ∈ S <;> simp only [hu, ↓reduceIte, vmap_idem_for_simp, ite_self]
 
-def QuotientInducedSubgraph.merge (G' : QuotientInducedSubgraph G) (v w : V) (hv : ¬G'.rmv v)
-  (hw : ∃ w', ∃ (h : (G'.vmap w').isSome = true), (G'.vmap w').get h = w) :
-    QuotientInducedSubgraph G where
-  rmv := G'.rmv
-  vmap u := if G'.vmap u = some v then some w else G'.vmap u
-  vmap_dom u := by
-    beta_reduce
-    split_ifs with h <;>
-    simp only [WithBot, vmap_dom, h, Option.isSome_some]
-  vmap_ran u hu := by
-    simp only at hu ⊢
-    split_ifs with h
-    · rcases hw with ⟨w', h', rfl⟩
-      rw [Option.get_some]
-      exact G'.vmap_ran w' ((G'.vmap_dom _).mpr h')
-    · exact G'.vmap_ran u hu
-  vmap_idem := fun u hu => by
-    simp only at hu ⊢
-    split_ifs with h
-    · simp only [Option.get_some, ite_eq_then]
-      intro hwv
-      rcases hw with ⟨w', hw', rfl⟩
-      rw [Option.some_get]
-      exact G'.vmap_idem w' ((G'.vmap_dom _).mpr hw')
-    · rw [G'.vmap_idem u hu]
-      simp only [h, ↓reduceIte]
+------------------------------------------------------------------------
+-- Lemmas about the elementary operations
+
+lemma Subgraph.not_mem_erm [DecidableEq E] [fullGraph G] (G' : Subgraph G) (e : E) :
+    let G'' := G'.erm e
+    ¬ (e ∈ G''.Eset ∧ (G.inc e).all (· ∈ G''.Vset)) := by
+  simp only [all_iff, decide_eq_true_eq, not_and, not_forall, Classical.not_imp]
+  rintro h
+
+  sorry
+
+-- def deleteEdges (G: Graph V E) (S : Set E) [DecidablePred (· ∈ S)] : Subgraph G :=
+--   (Subgraph.init G).OnSetE Sᶜ
+
 
 end Graph
